

DXXXXXXXXXXXXX
XIXXXXXXXXXXXXX
XXAXXXXXXXXXXXXX
XXXGXXXXXXXXXXXX
XXXOXXXXXXXXXXXX
XXXXNXXXXXXXXXX
XXXXXXAXXXXXXXXX
XXXXXXXLXXXXXXX
XXXXXXXXIXXXXXX
XXXXXXXXXSXXXXX
XXXXXXXXXXAXXXX
XXXXXXXXXXXXTXXX
XXXXXXXXXXXXIXX
XXXXXXXXXXXXOX
XXXXXXXXXXXXNX

Diagonalisation

The Road to Infinities, Truth and Gödel

Rasmus Bakken — Mahin Hossain

University of Oxford

Michaelmas 2025

Summary: We introduce provability inside a formal system, prove Gödel's diagonal lemma, and use it to show the undefinability of truth in a formal logical setting.

“All Cretans are liars.”

— EPIMENIDES, A CRETAN

Lecture 3 Summary

- What is a proof: define Hilbert-style system and axioms; example derivations.
- The Diagonal Lemma: construction of self-referential sentences via substitution and the diagonal operator.
- Undefinability of truth (Tarski): apply diagonal lemma to rule out a truth-defining formula in \mathcal{L} .

Roadmap

1 What is a Proof?

2 The Diagonal Lemma

3 The Undefinability of Truth

Motivating the concept

- From last time: a proof of φ_k is finite sequence of \mathcal{L} -formulas $\varphi_1, \dots, \varphi_k$ with some condition.

Motivating the concept

- From last time: a proof of φ_k is finite sequence of \mathcal{L} -formulas $\varphi_1, \dots, \varphi_k$ with some condition.
- The relevant condition: for all $1 \leq i \leq k$
 - φ_i is an axiom, or

Motivating the concept

- From last time: a proof of φ_k is finite sequence of \mathcal{L} -formulas $\varphi_1, \dots, \varphi_k$ with some condition.
- The relevant condition: for all $1 \leq i \leq k$
 - φ_i is an axiom, or
 - φ_i follows from φ_j and φ_m by some rule of inference where $j \leq m < i$.
- We use a Hilbert-style calculus.

Motivating the concept

- From last time: a proof of φ_k is finite sequence of \mathcal{L} -formulas $\varphi_1, \dots, \varphi_k$ with some condition.
- The relevant condition: for all $1 \leq i \leq k$
 - φ_i is an axiom, or
 - φ_i follows from φ_j and φ_m by some rule of inference where $j \leq m < i$.
- We use a Hilbert-style calculus.
- Logical vs non-logical axioms, and only two rules of inference.

Definition (First-order Predicate Logic)

Let φ , ψ and ξ be \mathcal{L} formula, then the following are axioms of first-order logic:

C1 $\varphi \rightarrow (\psi \rightarrow \varphi).$

C2 $(\varphi \rightarrow (\psi \rightarrow \xi)) \rightarrow ((\varphi \rightarrow \psi) \rightarrow (\varphi \rightarrow \xi)).$

C3 $(\varphi \rightarrow \psi) \rightarrow (\neg\psi \rightarrow \neg\varphi).$

Definition (First-order Predicate Logic)

Let φ , ψ and ξ be \mathcal{L} formula, then the following are axioms of first-order logic:

C1 $\varphi \rightarrow (\psi \rightarrow \varphi)$.

C2 $(\varphi \rightarrow (\psi \rightarrow \xi)) \rightarrow ((\varphi \rightarrow \psi) \rightarrow (\varphi \rightarrow \xi))$.

C3 $(\varphi \rightarrow \psi) \rightarrow (\neg\psi \rightarrow \neg\varphi)$.

C4 $\forall v_i \varphi(v_i) \rightarrow \varphi(t)$, where t is a term of \mathcal{L} such that it does not contain a variable v_j where v_i occurs free in the scope of $\forall v_j$ in φ .

C5 $\forall v_i (\varphi \rightarrow \psi) \rightarrow (\varphi \rightarrow \forall v_i \psi)$, provided v_i does not occur free in ψ .

C6 $\forall v_i (v_i = v_i)$.

C7 If F and G are atomic formulae, where G results from replacing some but not necessarily all of v_i in F by v_j , then $\forall v_i \forall v_j (v_i = v_j \rightarrow (F \rightarrow G))$ is an axiom.

Rules of Inference

Definition

The rules of inference are the following:

MP From φ and $\varphi \rightarrow \psi$ you may infer ψ .

Gen From φ you may infer $\forall v_i \varphi$.

Example: proving $\varphi \rightarrow \varphi$

$$\mathbf{1} \quad (\varphi \rightarrow ((\varphi \rightarrow \varphi) \rightarrow \varphi)) \rightarrow ((\varphi \rightarrow (\varphi \rightarrow \varphi)) \rightarrow (\varphi \rightarrow \varphi)) \quad \text{C2}$$

Example: proving $\varphi \rightarrow \varphi$

1 $(\varphi \rightarrow ((\varphi \rightarrow \varphi) \rightarrow \varphi)) \rightarrow ((\varphi \rightarrow (\varphi \rightarrow \varphi)) \rightarrow (\varphi \rightarrow \varphi))$ C2

2 $\varphi \rightarrow ((\varphi \rightarrow \varphi) \rightarrow \varphi)$ C1

Example: proving $\varphi \rightarrow \varphi$

- 1 $(\varphi \rightarrow ((\varphi \rightarrow \varphi) \rightarrow \varphi)) \rightarrow ((\varphi \rightarrow (\varphi \rightarrow \varphi)) \rightarrow (\varphi \rightarrow \varphi))$ C2
- 2 $\varphi \rightarrow ((\varphi \rightarrow \varphi) \rightarrow \varphi)$ C1
- 3 $((\varphi \rightarrow (\varphi \rightarrow \varphi)) \rightarrow (\varphi \rightarrow \varphi))$ MP line 1 and line 2

Example: proving $\varphi \rightarrow \varphi$

- 1 $(\varphi \rightarrow ((\varphi \rightarrow \varphi) \rightarrow \varphi)) \rightarrow ((\varphi \rightarrow (\varphi \rightarrow \varphi)) \rightarrow (\varphi \rightarrow \varphi))$ C2
- 2 $\varphi \rightarrow ((\varphi \rightarrow \varphi) \rightarrow \varphi)$ C1
- 3 $((\varphi \rightarrow (\varphi \rightarrow \varphi)) \rightarrow (\varphi \rightarrow \varphi))$ MP line 1 and line 2
- 4 $\varphi \rightarrow (\varphi \rightarrow \varphi)$ C1

Example: proving $\varphi \rightarrow \varphi$

- 1 $(\varphi \rightarrow ((\varphi \rightarrow \varphi) \rightarrow \varphi)) \rightarrow ((\varphi \rightarrow (\varphi \rightarrow \varphi)) \rightarrow (\varphi \rightarrow \varphi))$ C2
- 2 $\varphi \rightarrow ((\varphi \rightarrow \varphi) \rightarrow \varphi)$ C1
- 3 $((\varphi \rightarrow (\varphi \rightarrow \varphi)) \rightarrow (\varphi \rightarrow \varphi))$ MP line 1 and line 2
- 4 $\varphi \rightarrow (\varphi \rightarrow \varphi)$ C1
- 5 $\varphi \rightarrow \varphi$ MP line 3 and 4

Peano Arithmetic

Definition (Peano Arithmetic)

Peano Arithmetic, or *PA* for short, is the theory given by the following set of axioms:

PA1 $\forall v_i (S(v_i) \neq 0)$.

PA2 $\forall v_i \forall v_j (S(v_i) = S(v_j) \rightarrow v_i = v_j)$.

Peano Arithmetic

Definition (Peano Arithmetic)

Peano Arithmetic, or *PA* for short, is the theory given by the following set of axioms:

PA1 $\forall v_i (S(v_i) \neq 0).$

PA2 $\forall v_i \forall v_j (S(v_i) = S(v_j) \rightarrow v_i = v_j).$

PA3 $\forall v_i (v_i + 0 = v_i).$

PA4 $\forall v_i \forall v_j (v_i + S(v_j) = S(v_i + v_j)).$

Peano Arithmetic

Definition (Peano Arithmetic)

Peano Arithmetic, or *PA* for short, is the theory given by the following set of axioms:

PA1 $\forall v_i (S(v_i) \neq 0).$

PA2 $\forall v_i \forall v_j (S(v_i) = S(v_j) \rightarrow v_i = v_j).$

PA3 $\forall v_i (v_i + 0 = v_i).$

PA4 $\forall v_i \forall v_j (v_i + S(v_j) = S(v_i + v_j)).$

PA5 $\forall v_i (v_i * 0 = 0).$

PA6 $\forall v_i \forall v_j (v_i * S(v_j) = v_i * v_j + v_i).$

Peano Arithmetic

Definition (Peano Arithmetic)

Peano Arithmetic, or *PA* for short, is the theory given by the following set of axioms:

PA1 $\forall v_i (S(v_i) \neq 0).$

PA2 $\forall v_i \forall v_j (S(v_i) = S(v_j) \rightarrow v_i = v_j).$

PA3 $\forall v_i (v_i + 0 = v_i).$

PA4 $\forall v_i \forall v_j (v_i + S(v_j) = S(v_i + v_j)).$

PA5 $\forall v_i (v_i * 0 = 0).$

PA6 $\forall v_i \forall v_j (v_i * S(v_j) = v_i * v_j + v_i).$

PA7 $\forall v_i (\exp(v_i, 0) = \bar{1}).$

PA8 $\forall v_i \forall v_j (\exp(v_i, S(v_j)) = \exp(v_i, v_j) * v_i).$

Peano Arithmetic

Definition (Peano Arithmetic)

Peano Arithmetic, or *PA* for short, is the theory given by the following set of axioms:

PA1 $\forall v_i (S(v_i) \neq 0).$

PA2 $\forall v_i \forall v_j (S(v_i) = S(v_j) \rightarrow v_i = v_j).$

PA3 $\forall v_i (v_i + 0 = v_i).$

PA4 $\forall v_i \forall v_j (v_i + S(v_j) = S(v_i + v_j)).$

PA5 $\forall v_i (v_i * 0 = 0).$

PA6 $\forall v_i \forall v_j (v_i * S(v_j) = v_i * v_j + v_i).$

PA7 $\forall v_i (\exp(v_i, 0) = \bar{1}).$

PA8 $\forall v_i \forall v_j (\exp(v_i, S(v_j)) = \exp(v_i, v_j) * v_i).$

Ind \mathcal{L} For any \mathcal{L} formula with exactly one free variable $\varphi(v_i)$,
 $(\varphi(0) \wedge \forall v_i (\varphi(v_i) \rightarrow \varphi(S(v_i)))) \rightarrow \forall v_i \varphi(v_i)$ is an axiom.

Example in PA: $\bar{1} + \bar{1} = \bar{2}$ (pt.1)

Theorem

$PA \vdash \bar{1} + \bar{1} = \bar{2}$.

Proof.

1 $\forall v_i \forall v_j (v_i + S(v_j) = S(v_i + v_j))$ PA4

Example in PA: $\bar{1} + \bar{1} = \bar{2}$ (pt.1)

Theorem

$PA \vdash \bar{1} + \bar{1} = \bar{2}$.

Proof.

- 1 $\forall v_i \forall v_j (v_i + S(v_j) = S(v_i + v_j))$ PA4
- 2 $\forall v_i \forall v_j (v_i + S(v_j) = S(v_i + v_j)) \rightarrow \forall v_j (S(0) + S(v_j) = S(S(0) + v_j))$
C4
- 3 $\forall v_j (S(0) + S(v_j) = S(S(0) + v_j))$ MP with line 1 and line 2

Example in PA: $\bar{1} + \bar{1} = \bar{2}$ (pt.1)

Theorem

$$PA \vdash \bar{1} + \bar{1} = \bar{2}.$$

Proof.

- 1 $\forall v_i \forall v_j (v_i + S(v_j) = S(v_i + v_j))$ PA4
- 2 $\forall v_i \forall v_j (v_i + S(v_j) = S(v_i + v_j)) \rightarrow \forall v_j (S(0) + S(v_j) = S(S(0) + v_j))$
C4
- 3 $\forall v_j (S(0) + S(v_j) = S(S(0) + v_j))$ MP with line 1 and line
2
- 4 $\forall v_j (S(0) + S(v_j) = S(S(0) + v_j)) \rightarrow S(0) + S(0) = S(S(0) + 0)$ C4
- 5 $S(0) + S(0) = S(S(0) + 0)$ MP with line 3 and 4



Example in PA: $\overline{1} + \overline{1} = \overline{2}$ (pt.2)

Theorem

$PA \vdash \overline{1} + \overline{1} = \overline{2}$.

Proof.

5 $S(0) + S(0) = S(S(0) + 0)$ MP with line 3 and 4

6 $\forall v_i (v_i + 0 = v_i)$ PA3

Example in PA: $\bar{1} + \bar{1} = \bar{2}$ (pt.2)

Theorem

$PA \vdash \bar{1} + \bar{1} = \bar{2}$.

Proof.

5 $S(0) + S(0) = S(S(0) + 0)$ MP with line 3 and 4

6 $\forall v_i (v_i + 0 = v_i)$ PA3

7 $\forall v_i (v_i + 0 = v_i) \rightarrow S(0) + 0 = S(0)$ C4

8 $S(0) + 0 = S(0)$ MP with line 6 and line
7



Example in PA: $\overline{1} + \overline{1} = \overline{2}$ (pt.3)

Theorem

$PA \vdash \overline{1} + \overline{1} = \overline{2}$.

Proof.

5 $S(0) + S(0) = S(S(0) + 0)$ MP with line 3 and 4

8 $S(0) + 0 = S(0)$ MP with line 6 and line
7

9 $\forall v_i \forall v_j (v_i = v_j \rightarrow (S(0) + S(0) = S(v_i) \rightarrow S(0) + S(0) = S(v_j)))$ C7

Example in PA: $\bar{1} + \bar{1} = \bar{2}$ (pt.3)

Theorem

$$PA \vdash \bar{1} + \bar{1} = \bar{2}.$$

Proof.

5 $S(0) + S(0) = S(S(0) + 0)$ MP with line 3 and 4

8 $S(0) + 0 = S(0)$ MP with line 6 and line
7

9 $\forall v_i \forall v_j (v_i = v_j \rightarrow (S(0) + S(0) = S(v_i) \rightarrow S(0) + S(0) = S(v_j)))$ C7

10 $\forall v_i \forall v_j (v_i = v_j \rightarrow (S(0) + S(0) = S(v_i) \rightarrow S(0) + S(0) = S(v_j))) \rightarrow \forall v_j (S(0) + 0 = v_j \rightarrow (S(0) + S(0) = S(S(0) + 0) \rightarrow S(0) + S(0) = S(v_j)))$ C4

11 $\forall v_j (S(0) + 0 = v_j \rightarrow (S(0) + S(0) = S(S(0) + 0) \rightarrow S(0) + S(0) = S(v_j)))$
MP line 9 and line 10



Example in PA: $\bar{1} + \bar{1} = \bar{2}$ (pt.4)

Theorem

$$PA \vdash \bar{1} + \bar{1} = \bar{2}.$$

Proof.

5 $S(0) + S(0) = S(S(0) + 0)$ MP with line 3 and 4

8 $S(0) + 0 = S(0)$ MP with line 6 and line
7

11 $\forall v_j (S(0) + 0 = v_j \rightarrow (S(0) + S(0) = S(S(0) + 0) \rightarrow S(0) + S(0) = S(v_j)))$
MP line 9 and line 10

Example in PA: $\bar{1} + \bar{1} = \bar{2}$ (pt.4)

Theorem

$PA \vdash \bar{1} + \bar{1} = \bar{2}$.

Proof.

5 $S(0) + S(0) = S(S(0) + 0)$ MP with line 3 and 4

8 $S(0) + 0 = S(0)$ MP with line 6 and line
7

11 $\forall v_j (S(0) + 0 = v_j \rightarrow (S(0) + S(0) = S(S(0) + 0) \rightarrow S(0) + S(0) = S(v_j)))$
MP line 9 and line 10

12 $\forall v_j (S(0) + 0 = v_j \rightarrow (S(0) + S(0) = S(S(0) + 0) \rightarrow S(0) + S(0) = S(v_j))) \rightarrow S(0) + 0 = S(0) \rightarrow (S(0) + S(0) = S(S(0))) \rightarrow S(0) + S(0) = S(S(0)))$ C4

13 $S(0) + 0 = S(0) \rightarrow (S(0) + S(0) = S(S(0) + 0) \rightarrow S(0) + S(0) = S(S(0)))$
MP line 11 and line 12

Example in PA: $\bar{1} + \bar{1} = \bar{2}$ (pt.4)

Theorem

$$PA \vdash \bar{1} + \bar{1} = \bar{2}.$$

Proof.

5 $S(0) + S(0) = S(S(0) + 0)$ MP with line 3 and 4

8 $S(0) + 0 = S(0)$ MP with line 6 and line
7

11 $\forall v_j (S(0) + 0 = v_j \rightarrow (S(0) + S(0) = S(S(0) + 0) \rightarrow S(0) + S(0) = S(v_j)))$
MP line 9 and line 10

12 $\forall v_j (S(0) + 0 = v_j \rightarrow (S(0) + S(0) = S(S(0) + 0) \rightarrow S(0) + S(0) = S(v_j))) \rightarrow S(0) + 0 = S(0) \rightarrow (S(0) + S(0) = S(S(0))) \rightarrow S(0) + S(0) = S(S(0)))$ C4

13 $S(0) + 0 = S(0) \rightarrow (S(0) + S(0) = S(S(0) + 0) \rightarrow S(0) + S(0) = S(S(0)))$
MP line 11 and line 12

14 $(S(0) + S(0) = S(S(0) + 0) \rightarrow S(0) + S(0) = S(S(0)))$ MP line 8 and line 13

Example in PA: $\bar{1} + \bar{1} = \bar{2}$ (pt.5)

Theorem

$PA \vdash \bar{1} + \bar{1} = \bar{2}$.

Proof.

5 $S(0) + S(0) = S(S(0) + 0)$ MP with line 3 and 4

14 $(S(0) + S(0) = S(S(0) + 0) \rightarrow S(0) + S(0) = S(S(0)))$ MP line 8 and line 13

15 $S(0) + S(0) = S(S(0))$ MP line 5 and line 14



Roadmap

1 What is a Proof?

2 The Diagonal Lemma

3 The Undefinability of Truth

Gödel's Diagonal Lemma

Diagonal Lemma

If $\varphi(v_n)$ is an \mathcal{L} -formula with one free variable, then there is an \mathcal{L} -sentence γ such that

$$PA \vdash \gamma \leftrightarrow \varphi(\ulcorner \gamma \urcorner).$$

- For any one-place formula, we can manufacture a sentence that says of itself that it has property φ .
- This turns Gödel codes + substitution into genuine *self-reference*.

Substitution on Formulae

- Given a formula φ and a term t , $\varphi(t/v_i)$ means:
 - uniformly replace all *free* occurrences of v_i in φ by t .
- Example: φ is $S(v_5) = S(S(0))$.
 - $\varphi(S(0)/v_5)$ is $S(S(0)) = S(S(0))$.
 - $\varphi(0/v_5)$ is $S(0) = S(S(0))$.
 - $\varphi(v_3/v_5)$ is $S(v_3) = S(S(0))$.
- Beware **variable capture**:
 - quantifiers can accidentally bind new free variables,
 - we avoid this by renaming bound variables before substituting.

Internalising Substitution: The Function *sub*

Lemma (informal)

There is an \mathcal{L} -definable function $sub(v_1, v_2, v_3)$ such that

$$PA \vdash \overline{\varphi} = sub(\overline{\psi}, \overline{n}, \overline{t})$$

iff $\varphi = \psi(t/v_n)$.

- So substitution on formulas can be mirrored by a calculation on Gödel numbers.
- We take the existence of such a *sub*-function for granted (construction is tedious but standard).

The Diagonal Operator

Definition (Diagonal Operator)

Let $\varphi(v_n)$ be a formula with v_n its only free variable. Define

$$\text{dia}(\overline{\ulcorner \varphi(v_n) \urcorner}) := \text{sub}(\overline{\ulcorner \varphi \urcorner}, \overline{n}, \overline{\overline{\ulcorner \varphi \urcorner}}).$$

- Intuition:

$$\text{dia}(\overline{\ulcorner \varphi \urcorner}) = \overline{\ulcorner \varphi(\overline{\ulcorner \varphi \urcorner} / v_n) \urcorner}.$$

- It takes the code of φ and returns the code of the result of plugging that very code back into φ .
- This is the core mechanism behind self-reference.

Proof Idea of the Diagonal Lemma

- Fix a formula $\varphi(v_n)$.
- Consider the auxiliary formula

$$\theta(v_n) := \exists x (x = \text{dia}(v_n) \wedge \varphi(x)).$$

- Now look at the sentence

$$\gamma := \exists x (x = \text{dia}(\overline{\ulcorner \theta \urcorner}) \wedge \varphi(x)).$$

- Using the properties of *sub* and *dia*, one checks inside *PA* that

$$\text{dia}(\overline{\ulcorner \theta \urcorner}) = \overline{\ulcorner \gamma \urcorner}.$$

- Hence *PA* proves

$$\gamma \leftrightarrow \varphi(\overline{\ulcorner \gamma \urcorner}),$$

which is exactly the conclusion of the Diagonal Lemma.

Roadmap

1 What is a Proof?

2 The Diagonal Lemma

3 The Undefinability of Truth

What Should a Truth Predicate Do?

- Suppose $\varphi(v_i)$ is meant to say:

$$\varphi(\ulcorner \psi \urcorner) = \text{"}\psi \text{ is true"}$$

- We would like φ to respect logical structure, e.g. disjunction:

$$PA \vdash \varphi(\ulcorner \psi_1 \vee \psi_2 \urcorner) \leftrightarrow \varphi(\ulcorner \psi_1 \urcorner) \vee \varphi(\ulcorner \psi_2 \urcorner).$$

- More strongly: there is a coding function $x \dot{\vee} y$ with

$$x = \ulcorner \psi_1 \urcorner, y = \ulcorner \psi_2 \urcorner \Rightarrow x \dot{\vee} y = \ulcorner \psi_1 \vee \psi_2 \urcorner,$$

and we might want

$$PA \vdash \forall x \forall y (\varphi(x \dot{\vee} y) \leftrightarrow \varphi(x) \vee \varphi(y)).$$

Tarski Biconditionals (for φ)

For every \mathcal{L} -sentence ψ ,

$$PA \vdash \varphi(\overline{\ulcorner \psi \urcorner}) \leftrightarrow \psi.$$

- This is a very natural *minimal* requirement for a truth definition.
- Read: “ φ holds of the code of ψ iff ψ .”
- Tarski’s theorem: no such φ exists in the language of PA .

Tarski's Undefinability Theorem

Theorem (Tarski)

There is no \mathcal{L} -formula $\varphi(v_i)$ such that for all \mathcal{L} -sentences ψ ,

$$PA \vdash \varphi(\overline{\ulcorner \psi \urcorner}) \leftrightarrow \psi.$$

- So: the intuitive notion of *truth in the standard model of PA* is not arithmetically definable.
- This contrasts with many other notions (e.g. “even”, “provable in PA ”) which *are* definable in \mathcal{L} .

Proof Idea: The Liar Sentence

Proof sketch

Assume, for contradiction, that such a $\varphi(v_i)$ exists.

- Apply the Diagonal Lemma to $\neg\varphi(v_i)$.
- Obtain a sentence λ such that

$$PA \vdash \lambda \leftrightarrow \neg\varphi(\ulcorner \lambda \urcorner).$$

- But by the Tarski biconditionals we also have

$$PA \vdash \lambda \leftrightarrow \varphi(\ulcorner \lambda \urcorner).$$

- Combining:

$$PA \vdash \lambda \leftrightarrow \neg\lambda,$$

contradicting the consistency of PA .

The Liar and Beyond

- The sentence λ above is a formal **liar sentence**:

λ says “I am not true (w.r.t. φ)”.

- Tarski’s theorem shows:
 - No \mathcal{L} -formula can define a fully adequate truth predicate for arithmetic.
 - Truth is strictly more complex than many other arithmetical properties.
- One response: extend the language with a new primitive truth predicate T .
- Example theory:

$$TB := PA \cup \{ T^{\overline{\ulcorner \psi \urcorner}} \leftrightarrow \psi \mid \psi \text{ an } \mathcal{L}\text{-sentence} \}.$$

- The liar reappears, but now at the *extended* level, and must be handled with care.